src/QueryEq.v
@@ -1,3 +1,4 @@
+Require Import List.
 From mathcomp Require Import all_ssreflect.
 Set Implicit Arguments.
 Unset Strict Implicit.
@@ -23,83 +24,87 @@ Require Import QueryConformance.
 Require Import QuerySemantic.
 Require Import NRGTNF.
 
+Require Import String.
+
 Section Eq.
 
   Variables N Name Vals : ordType.
   Implicit Type schema : @wfSchema Name Vals.
 
-  Inductive Correct schema : @QuerySet Name Vals -> (@NamedType Name * @NamedType Name) -> Prop :=
-  | CSQ : forall ϕ root current,
-      Correct' schema ϕ (root, current) ->
-      Correct schema (SingleQuery ϕ) (root, current)
-              
-  | CSS : forall ϕ ϕ' root current,
-      Correct' schema ϕ (root, current) ->
-      Correct schema ϕ' (root, current) ->
-      Correct schema (SelectionSet ϕ ϕ') (root, current)
-              
-  with Correct' schema : Query -> (NamedType * NamedType) -> Prop :=
-       | CF : forall f α root current,
-           Correct' schema (SingleField f α) (root, current)
+  Inductive Correct schema : (NamedType * NamedType) -> Query -> Prop :=
+  | CF : forall f α root current,
+      query_conforms schema current (SingleField f α) ->
+      Correct schema (root, current) (SingleField f α)
 
-       | CLF : forall l f α root current,
-           Correct' schema (LabeledField l f α) (root, current)
+  | CLF : forall l f α root current,
+      query_conforms schema current (LabeledField l f α) ->
+      Correct schema (root, current) (LabeledField l f α)
+               
+  | CNF : forall f α ϕ root current ty',
+      query_conforms schema current (NestedField f α ϕ) ->
+      lookup_field_type schema current f = Some ty' ->
+      Forall (Correct schema (name_of_type ty', name_of_type ty')) ϕ ->
+      Correct schema (root, current) (NestedField f α ϕ) 
+               
+  | CNLF : forall l f α ϕ root current ty',
+      query_conforms schema current (NestedLabeledField l f α ϕ) ->
+      lookup_field_type schema current f = Some ty' ->
+      Forall (Correct schema (name_of_type ty', name_of_type ty')) ϕ ->
+      Correct schema (root, current) (NestedLabeledField l f α ϕ) 
 
-       | CNF : forall f α ϕ root current ty',
-           lookup_field_type schema root f = Some ty' ->
-           Correct schema ϕ (name_of_type ty', name_of_type ty') ->
-           Correct' schema (NestedField f α ϕ) (root, current)
-
-       | CNLF : forall l f α ϕ root current ty',
-           lookup_field_type schema root f = Some ty' ->
-           Correct schema ϕ (name_of_type ty', name_of_type ty') ->
-           Correct' schema (NestedLabeledField l f α ϕ) (root, current)
-
-       | CIF : forall root current t ϕ,
-           current \in get_possible_types schema t ->
-           Correct schema ϕ (root, t) ->
-           Correct' schema (InlineFragment t ϕ) (root, current).
+  | CIF_SS : forall t t' ϕ,  (* This includes the case when t = t' *)
+      query_conforms schema t' (InlineFragment t ϕ) ->
+      t \in get_possible_types schema t' ->
+            Forall (Correct schema (t', t)) ϕ ->
+            Correct schema (t', t') (InlineFragment t ϕ)   
                     
-         
-  Lemma Correct_SQE schema ϕ ty : Correct schema (SingleQuery ϕ) ty ->
-                                  Correct' schema ϕ ty.
-  Proof. by move=> H; inversion H. Qed.
-
-  Lemma Correct_SSE schema ϕ ϕ' ty : Correct schema (SelectionSet ϕ ϕ') ty ->
-                                     Correct' schema ϕ ty /\ Correct schema ϕ' ty.
-  Proof. by move=> H; inversion H. Qed.
-
-  Definition QueryEq schema (g : @conformedGraph N Name Vals schema) (q1 q2 : QuerySet)  :=
-    query_set_conforms schema q1 schema.(query_type) ->
-    query_set_conforms schema q2 schema.(query_type) ->
-    eval schema g g.(root) q1 = eval schema g g.(root) q2.
+  | CIF_ST : forall t t' ϕ,
+      query_conforms schema t (InlineFragment t ϕ) ->
+      Forall (Correct schema (t', t)) ϕ ->
+      Correct schema (t', t) (InlineFragment t ϕ)
+                    
+  | CIF_TT' : forall t t' ϕ,
+      query_conforms schema t (InlineFragment t' ϕ) ->
+      Forall (Correct schema (t, t')) ϕ ->
+      Correct schema (t, t) (InlineFragment t' ϕ)
+               
+  | CIF_TS' : forall t t' ϕ,
+      query_conforms schema t' (InlineFragment t' ϕ) ->
+      Forall (Correct schema (t, t')) ϕ ->
+      Correct schema (t, t') (InlineFragment t' ϕ)
+               
+  | CIF_TS : forall t t' ϕ,
+      query_conforms schema t' (InlineFragment t ϕ) ->
+      Forall (Correct schema (t, t)) ϕ ->
+      Correct schema (t, t') (InlineFragment t ϕ).
+  Set Elimination Schemes.
 
   
 
-  Lemma inline_eq schema (g : @conformedGraph N Name Vals schema) : forall t ϕ,
-      eval_query schema g g.(root) (InlineFragment t ϕ) = eval_query schema g g.(root) (InlineFragment t (SingleQuery (InlineFragment t ϕ))).
-  Proof.
-    move=> t ϕ; rewrite /eval_query /=.
-    case: lookup_type => //.
-    case=> //.
-    by move=> *; case: eqP.
-    by move=> *; case: declares_implementation.
-    by move=> *; case: (_ \in _).
-  Qed.
+  Definition QueryEq schema (g : @conformedGraph N Name Vals schema) u ty (q1 q2 : Query)  :=
+    query_conforms schema ty q1 ->
+    query_conforms schema ty q2 ->
+    eval schema g u q1 = eval schema g u q2.
+
+  Definition QueriesEq schema (g : @conformedGraph N Name Vals schema) u ty (q1 q2 : seq Query) :=
+    queries_conform schema ty q1 ->
+    queries_conform schema ty q2 ->
+    eval_queries schema g u q1 = eval_queries schema g u q2.
+    
 
   Lemma inline_nested_empty schema (g : @conformedGraph N Name Vals schema) :
     forall t1 t2 ϕ,
       is_object_type schema t1 ->
       is_object_type schema t2 ->
       t1 <> t2 ->
-      eval_query schema g g.(root) (InlineFragment t1 (SingleQuery (InlineFragment t2 ϕ))) = inr (Results [::]).
+      eval schema g g.(root) (InlineFragment t1 [:: (InlineFragment t2 ϕ)]) = [::].
   Proof.
     move=> t1 t2 ϕ.
     funelim (is_object_type schema t1) => //.
     funelim (is_object_type schema0 t2) => //.
     move=> _ _ Hdiff.
-    rewrite /eval_query Heq0.
-    case: eqP => // <-.
+    rewrite /eval Heq0.
+    case: eqP => //= <-.
     rewrite Heq.
     by case: eqP => // Ht1t2; rewrite Ht1t2 in Hdiff.
   Qed.
@@ -107,7 +112,7 @@ Section Eq.
   Lemma inline_query_preserves schema (g : @conformedGraph N Name Vals schema):
     forall ϕ u,
       u \in nodes g.(graph) ->
-      eval_query schema g u ϕ = eval_query schema g u (InlineFragment u.(type) (SingleQuery ϕ)).
+      eval schema g u ϕ = eval schema g u (InlineFragment u.(type) [:: ϕ]).
   Proof.
     move=> ϕ u Hin; case: g Hin.
     move=> g Hr He Hf Hn /= Hin.
@@ -115,29 +120,13 @@ Section Eq.
     move/seq.allP /(_ u Hin): Hn.
     case: u Hin => id ty flds Hin. rewrite /type. funelim (is_object_type schema ty) => //.
     move=> _.
+    rewrite Heq.
     case: ϕ.
-    move=> name α. rewrite /eval_query. rewrite Heq.
+    move=> name α. rewrite /eval. 
     simpl.  Admitted.
 
     
 
-
-  Fixpoint query_set_of_list (s : seq Query) : option (@QuerySet Name Vals) :=
-    match s with
-    | [::] => None
-    | hd :: [::] => Some (SingleQuery hd)
-    | hd :: tl => if query_set_of_list tl is Some q then
-                   Some (SelectionSet hd q)
-                 else
-                   None
-    end.
-
-  Equations append_queries (qs1 qs2 : @QuerySet Name Vals) : @QuerySet Name Vals :=
-    {
-      append_queries (SingleQuery q1) q2 := SelectionSet q1 q2;
-      append_queries (SelectionSet q1 q1') q2 := SelectionSet q1 (append_queries q1' q2)
-
-    }.
 
   Lemma filter_preserves T (p pred : T -> bool) (s : seq T) :
     seq.all p s ->
@@ -151,68 +140,36 @@ Section Eq.
   Qed.
 
   
-    
-  
-  Inductive QueryRed (schema : @wfSchema Name Vals) : QuerySet -> QuerySet -> Prop :=
-  | SQ1 : forall ϕ ϕ',
-      AtomicQueryRed schema ϕ ϕ' ->
-      QueryRed schema (SingleQuery ϕ) (SingleQuery ϕ')
-
+  Inductive QueryRed (schema : @wfSchema Name Vals) : seq Query -> seq Query -> Prop :=
   | SS1 : forall ϕ ϕ' ϕs,
       AtomicQueryRed schema ϕ ϕ' ->
-      QueryRed schema (SelectionSet ϕ ϕs) (SelectionSet ϕ' ϕs)
+      QueryRed schema [:: ϕ ; ϕs] [:: ϕ' ; ϕs]
                    
-  | SF_None : forall (ϕ : @QuerySet Name Vals) n α,
-      filter (predC1 (SingleField n α)) ϕ == None ->
-      QueryRed schema (SelectionSet (SingleField n α) ϕ) (SingleQuery (SingleField n α))
+  | SF_None : forall (ϕ ϕ' : seq (@Query Name Vals)) n α,
+      let ϕ' := filter (predC1 (SingleField n α)) ϕ in
+      QueryRed schema ((SingleField n α) :: ϕ) ((SingleField n α) :: ϕ')
 
-  | SF_Some : forall (ϕ ϕ' : @QuerySet Name Vals) n α,
-      filter (predC1 (SingleField n α)) ϕ == Some ϕ' ->
-      QueryRed schema (SelectionSet (SingleField n α) ϕ) (SelectionSet (SingleField n α) ϕ')
+  | LF_Some : forall (ϕ ϕ' : seq (@Query Name Vals)) l n α,
+      let ϕ' := filter (predC1 (LabeledField l n α)) ϕ in
+      QueryRed schema ((LabeledField l n α) :: ϕ) ((LabeledField l n α) :: ϕ')
 
-
-  | LF_None :  forall (ϕ : @QuerySet Name Vals) l n α,
-      filter (predC1 (LabeledField l n α)) ϕ == None ->
-      QueryRed schema
-               (SelectionSet (LabeledField l n α) ϕ)
-               (SingleQuery (LabeledField l n α))
-
-  | LF_Some : forall (ϕ ϕ' : @QuerySet Name Vals) l n α,
-      filter (predC1 (LabeledField l n α)) ϕ == Some ϕ' ->
-      QueryRed schema
-               (SelectionSet (LabeledField l n α) ϕ)
-               (SelectionSet (LabeledField l n α) ϕ')
-
-  | NF_None : forall (ϕ β χ : @QuerySet Name Vals) (n : Name) (α α' : {fmap Name -> Vals}),
+  | NF_Some : forall (ϕ ϕ' β : seq (@Query Name Vals)) (n : Name) (α α' : {fmap Name -> Vals}),
       let subqueries := foldr (fun q acc => if q is NestedField n' α' χ then
                                           if (n' == n) && (α == α') then
-                                            append_queries acc χ
+                                            χ ++ acc
                                           else
                                             acc
                                         else
-                                          acc) β ϕ
+                                          acc) [::] ϕ
       in
-      (filter (fun q => ~~(partial_query_eq (NestedField n α β) q)) ϕ) == None ->
-      QueryRed schema (SelectionSet (NestedField n α β) ϕ)
-                      (SingleQuery (NestedField n α subqueries))
-               
-  | NF_Some : forall (ϕ ϕ' β χ : @QuerySet Name Vals) (n : Name) (α α' : {fmap Name -> Vals}),
-      let subqueries := foldr (fun q acc => if q is NestedField n' α' χ then
-                                          if (n' == n) && (α == α') then
-                                            append_queries acc χ
-                                          else
-                                            acc
-                                        else
-                                          acc) β ϕ
-      in
-      (filter (fun q => ~~(partial_query_eq (NestedField n α β) q)) ϕ) == Some ϕ' ->
-      QueryRed schema (SelectionSet (NestedField n α β) ϕ)
-                      (SelectionSet (NestedField n α subqueries) ϕ')
+      let ϕ' := (filter (fun q => ~~(partial_query_eq (NestedField n α β) q)) ϕ) in 
+      QueryRed schema ((NestedField n α β) :: ϕ)
+                      ((NestedField n α (β ++ subqueries)) :: ϕ')
                
                 
   | Inline_spread : forall t ϕ ϕ',
-      QueryRed schema (SingleQuery (InlineFragment t (SelectionSet ϕ ϕ')))
-                      (SelectionSet (InlineFragment t (SingleQuery ϕ)) (SingleQuery (InlineFragment t ϕ')))
+      QueryRed schema [:: (InlineFragment t  (ϕ :: ϕ'))]
+                      [:: (InlineFragment t [:: ϕ]) ; (InlineFragment t ϕ')]
         
 
   with
@@ -233,7 +190,7 @@ Section Eq.
       AtomicQueryRed schema (InlineFragment t ϕ) (InlineFragment t ϕ')
 
   | Inline_nested : forall t ϕ,
-      AtomicQueryRed schema (InlineFragment t (SingleQuery (InlineFragment t ϕ))) (InlineFragment t ϕ) 
+      AtomicQueryRed schema (InlineFragment t [:: InlineFragment t ϕ]) (InlineFragment t ϕ) 
 
   | AQR_Inline_Int : forall t t1 ϕ,
       t \in implementation schema t1 ->
@@ -251,16 +208,6 @@ Section Eq.
   Proof. by move=> H; inversion H. Qed.
 
   
-                                                             
-  Lemma normal_form_fld_inline (query_set : @QuerySet Name Vals) : is_ground_typed_normal_form query_set ->
-                                                                   (forall q : Query, in_query q query_set -> is_field q) \/ (forall q : Query, in_query q query_set -> is_inline_fragment q).
-  Proof.
-    case: query_set => [q | q qs].
-    - case: q=> //=; do ?[by move=> *; left => q; move/eqP <-].
-      by move=> *; right => q'; move/eqP <-.
-    - rewrite is_ground_typed_normal_form_equation_2.
-        by move/and3P=> [/orP [Hf | Hi] _ _]; [left | right]; apply/allP.
-  Qed.
 
 
   Lemma filter_all_predC1 (T : eqType) (s : seq T) (x : T) :
@@ -273,6 +220,7 @@ Section Eq.
   Qed.
 
 
+  (*
   Lemma query_filter_preserves (queries ϕ' : @QuerySet Name Vals) p pred :
     all pred queries -> filter p queries = Some ϕ' -> all pred ϕ'.
   Proof.
@@ -297,8 +245,9 @@ Section Eq.
     - by move=> n f ϕ H q /allP H'; apply: H'.
     - by move=> l n f ϕ H q /allP H'; apply: H'.
     - by move=> t ϕ H q /allP H'; apply: H'.
-  Qed.
+  Qed. *)
 
+  (*
   Lemma filter_preserves_normal (queries ϕ' : @QuerySet Name Vals) p :
     is_ground_typed_normal_form queries ->
     filter p queries = Some ϕ' ->
@@ -318,31 +267,221 @@ Section Eq.
       rewrite is_ground_typed_normal_form_equation_2.
       move: (Hq' sm Hnf' Hfilt).
   Admitted.
-
+*)
+(*
   Lemma filter_preserves_non_redundancy (queries ϕ' : @QuerySet Name Vals) p :
     is_non_redundant queries ->
     filter p queries = Some ϕ' ->
     is_non_redundant ϕ'.
   Proof.
     Admitted.
-      
-  Theorem all_q_has_nrgtnf_q schema (g : @conformedGraph N Name Vals schema) :
-    forall  (ϕ : @QuerySet Name Vals),
-      Correct schema ϕ (schema.(query_type), schema.(query_type)) ->
-      exists (ϕ' : @QuerySet Name Vals),
-        [/\ is_ground_typed_normal_form ϕ' ,
-         is_non_redundant ϕ' ,
-         QueryRed schema ϕ ϕ' &
-         QueryEq g ϕ ϕ'].
+*)
+
+  Lemma queries_conform_cons schema ty hd tl :
+    queries_conform schema ty (hd :: tl) -> query_conforms schema ty hd.
   Proof.
+    rewrite /queries_conform.
+      by move/andP=> [_ /= /andP [Hhd _]].
+  Qed.
+
+  Lemma correct_conforms schema root current ϕ :
+    Correct schema (root, current) ϕ ->
+    query_conforms schema current ϕ.
+  Proof.
+    move: root current.
+    elim ϕ using Query_ind with (Pl := fun qs => forall root current, qs != [::] -> Forall (Correct schema (root, current)) qs -> queries_conform schema current qs) => //.
+    by intros; inversion H.
+    by intros; inversion H.
+    by move=> n α ϕ' IH root current H; inversion H.  
+    by move=> l n α ϕ' IH root current H; inversion H.
+    by move=> t ϕ' IH root current H; inversion H.
+    move=> q IH qs IH' root current Hne H.
+    rewrite /queries_conform.
+    apply/andP; split => //.
+    simpl. apply/andP; split => //.
+    move: (Forall_cons_inv H) => [H1 H2].
+    apply: (IH _ _ H1).
+    case: qs IH' Hne H => //.
+    move=> hd tl H.
+    Admitted.
+
+  Lemma nested_conforms_list schema ty n α ϕ :
+    query_conforms schema ty (NestedField n α ϕ) -> ϕ != [::].
+  Proof.
+    simpl.
+    move/andP=> [/nilP H _]; case: eqP => //.
+  Qed.
+
+  Lemma not_nil_spread {A : eqType} (lst : seq A) : lst != [] -> exists x lst', lst = x :: lst'.
+  Proof.
+      by case: lst => // x lst' H; exists x; exists lst'.  Qed.
+  
+  Lemma single_field_correct schema ty ty' n α :
+    Correct schema (ty, ty') (SingleField n α).
+  Proof. apply: CF. Admitted.
+
+ 
+   
+  Lemma empty_queries_N_conform schema ty : ~ queries_conform schema ty [::].
+  Proof. done. Qed.
+
+  Lemma nf_queries_conform schema ty fld n α ϕ :
+    query_conforms schema ty (NestedField n α ϕ) ->
+    lookup_field_in_type schema ty n = Some fld ->
+    queries_conform schema fld.(return_type) ϕ.
+  Proof.
+    rewrite /query_conforms.
+    move/andP=> [/nilP HNnil Hlook].
+    case H : lookup_field_in_type => [fld'|] //.
+    case=> <-.
+    rewrite H in Hlook. move/andP: Hlook => [Hargs Hall].
+    rewrite -/(query_conforms schema fld') in Hall.
+    rewrite /queries_conform.
+    apply/andP. split.
+    rewrite /negb. case eqP => //. done.
+  Qed.
+
+  Lemma nf_conforms_lookup_some schema ty  n α ϕ :
+    query_conforms schema ty (NestedField n α ϕ) ->
+    exists fld, lookup_field_in_type schema ty n = Some fld.
+  Proof. rewrite /query_conforms.
+    move/andP=> [_].
+    case Hlook : lookup_field_in_type => [fld'|] //.
+    by exists fld'.
+  Qed.
+
+  Lemma nf_correct_lookup_some schema root current n α ϕ :
+    Correct schema (root, current) (NestedField n α ϕ) ->
+    exists fld, lookup_field_type schema current n = Some fld. 
+  Proof.
+    move=> H; inversion H.
+      by exists ty'.
+  Qed.
+    
+  Lemma nf_queries_conform' schema ty n α ϕ :
+    query_conforms schema ty (NestedField n α ϕ) ->
+    exists ty', queries_conform schema ty' ϕ.
+  Proof.
+    rewrite /query_conforms.
+    move/andP=> [/nilP HNnil Hlook].
+    move: Hlook.
+    case H : lookup_field_in_type => [fld'|] //.
+    move/andP=> [Hargs Hall].
+    rewrite -/(query_conforms schema fld') in Hall.
+    rewrite /queries_conform.
+    exists (fld'.(return_type)).
+    by apply/andP; split => //; case eqP. 
+  Qed.
+
+  Lemma nf_queries_conform'' schema ty n α ϕ fld :
+    lookup_field_in_type schema ty n = Some fld ->
+    query_conforms schema ty (NestedField n α ϕ) ->
+    queries_conform schema fld.(return_type) ϕ.
+  Proof.
+    move=> Hlook; rewrite /query_conforms.
+    move/andP=> [/nilP HNnil].
+    rewrite Hlook.
+    move/andP=> [_]. rewrite -/(query_conforms schema fld).
+    move=> Hall.
+    rewrite /queries_conform.
+      by apply/andP; split => //; case eqP.
+  Qed.
+    
+    
+  Lemma lookup_field_or_type schema lookup_type ty name fld :
+    lookup_field_in_type schema lookup_type name = Some fld ->
+    lookup_field_type schema lookup_type name = Some ty ->
+    ty = fld.(return_type).
+  Proof.
+    by rewrite /lookup_field_type; move=> ->; case. Qed.
+
+  Lemma nf_queries_correct schema root current n α ϕ fld :
+    lookup_field_type schema current n = Some fld ->
+    Correct schema (root, current) (NestedField n α ϕ) ->
+    Forall (Correct schema (name_of_type fld, name_of_type fld)) ϕ.
+  Proof.  by move=> Hlook H; inversion H; rewrite Hlook in H6; case: H6 => ->. Qed.
+
+
+  Lemma nf_queries_eq schema (g : @conformedGraph N Name Vals schema) u n α ϕ ϕ' :
+    (forall v, eval_queries schema g v ϕ = eval_queries schema g v ϕ') ->
+    eval schema g u (NestedField n α ϕ) = eval schema g u (NestedField n α ϕ').
+  Proof.
+    rewrite /eval_queries.
+    move=> Hqs.
+    rewrite /eval.
+    case lookup_field_type => //.
+    case=> [nt | lt].
+    case get_target_nodes_with_field => // v1 vn /=.
+    by rewrite -/(eval schema g v1); move: (Hqs v1) => ->. 
+    case get_target_nodes_with_field => // v1 vn /=.
+    rewrite -/(eval schema g v1). move: (Hqs v1) => ->.
+  Admitted.
+    
+
+  Theorem all_q_has_nrgtnf_q schema (g : @conformedGraph N Name Vals schema) u root (ϕ : @Query Name Vals):
+    u \in nodes g ->
+    query_conforms schema u.(type) ϕ ->
+    Correct schema (root, u.(type)) ϕ ->
+    exists (ϕ' : @Query Name Vals),
+      [/\ is_in_normal_form ϕ' ,
+       is_non_redundant ϕ' ,
+       AtomicQueryRed schema ϕ ϕ' &
+       QueryEq g u u.(type) ϕ ϕ'].
+  Proof.
+    elim ϕ using Query_ind with
+        (Pl := fun qs => forall v root,
+                  v \in nodes g ->
+                  queries_conform schema v.(type) qs ->
+                  Forall (Correct schema (root, v.(type))) qs ->    
+                  exists (qs' : seq Query),
+                    [/\ are_in_normal_form qs',
+                     are_non_redundant qs',
+                     QueryRed schema qs qs' &
+                     QueriesEq g v v.(type) qs qs']).
+    - by move=> n α; exists (SingleField n α); split => //; constructor.
+    - by move=> l n α; exists (LabeledField l n α); split => //; constructor.
+    - move=> n α qs IH Huin Hqc Hok.
+      move: (nf_conforms_lookup_some Hqc); case=> fld Hlook.
+      move: (nf_queries_conform'' Hlook Hqc) => Hqsc.
+      move: (nf_correct_lookup_some Hok); case=> ty' Hlook'.
+      move: (nf_queries_correct Hlook' Hok).
+      move: Hqsc.
+      move: (lookup_field_or_type Hlook Hlook') => <- Hqsc Hqsok.
+      pose target_nodes := get_target_nodes_with_field g u (Field n α).
+      case: ty' Hlook' Hqsc Hqsok => [nt | lt].
+      pose hd := ohead target_nodes.
+      move: IH. case=> v.
+      case=> qs' [Hnfs Hnrs Hreds Heqs].
+      exists (NestedField n α qs'); split => //=.
+      constructor. done.
+      rewrite /QueryEq. move=> _ Hqsc'.
+      rewrite /eval /=. rewrite Hlook'.
+      case ty'.
+      
+      
     move=> ϕ.
-    elim ϕ using QuerySet_ind with (P0 := fun q =>
-                                           Correct' schema q (schema.(query_type), schema.(query_type)) ->
-                                           exists q', [/\ is_query_in_normal_form q' , is_query_non_redundant q' ,
-                                                  AtomicQueryRed schema q q' &
-                                                  (query_conforms schema q schema.(query_type) ->
-                                                   query_conforms schema q' schema.(query_type) ->
-                                                   eval_query schema g g.(root) q = eval_query schema g g.(root) q')]).
+    elim: ϕ ty ty' => [//| hd tl IH] ty ty'.
+    case: tl IH.
+    move/(_ ty ty').
+    case=> //=. move: empty_queries_N_conform. move/(_ schema ty'). 
+    move/queries_conform_cons.
+    move=> ϕ; elim: ϕ ty ty'.
+    - by move=> n α ty ty' Hc; exists (SingleField n α); split => //; constructor.
+    - by move=> l n α ty ty' Hc; exists (LabeledField l n α); split => //; constructor.
+    - move=> n α ϕ.
+      move=> IH ty ty' Hc; move: (correct_conforms Hc) => Hcnfs.
+      move: (nested_conforms_list Hcnfs) => Hnnil.
+      move: (not_nil_spread Hnnil); case=> hd; case=> tl.
+      case: hd => n' α' H.
+      rewrite H in IH. move: (Forall_cons_inv IH) => [Hhd Htl].
+      rewrite H in Hc. inversion Hc.
+      move: (Forall_cons_inv H7) => [H'c H''].
+      move: (Hhd ty'0 ty'0 H'c).
+      rewrite H. move: (Hhd single_field_correct).
+      exists (NestedField n α ((SingleField n' α') :: (filter (predC1 (SingleField n' α')) tl))).
+      split => //=.
+      case: hd H IH Hhd.
+      
     - move=> q Hex /Correct_SQE /Hex; case=> q' [Hnf Hnr Hred Heq].
       exists (SingleQuery q'); split => //. 
       * by constructor.
