src/QueryAux.v
@@ -14,42 +14,24 @@ Section QueryAux.
 
   Variables Name Vals : ordType.
 
-  Implicit Type query_set : @QuerySet Name Vals.
+  Implicit Type queries : seq (@Query Name Vals).
   Implicit Type query : @Query Name Vals.
   Implicit Type response : @ResponseObject Name Vals.
-  Implicit Type result : @Result Name Vals.
 
-  (*
-  Equations query_set_size query_set : nat :=
+
+  Equations query_size query : nat :=
     {
-      query_set_size (SingleQuery q) := query_size q;
-      query_set_size (SelectionSet q q') := query_size q + query_set_size q'
+      query_size (NestedField _ _ q') := 1 + queries_size q';
+      query_size (NestedLabeledField _ _ _ q') => 1 + (queries_size q');
+      query_size (InlineFragment _ q') => 1 + (queries_size q');
+      query_size _ := 1
     }
   where
-  query_size query : nat :=
+  queries_size queries : nat :=
     {
-      query_size (NestedField _ _ q') := 1 + (query_set_size q');
-      query_size (NestedLabeledField _ _ _ q') := 1 + (query_set_size q');
-      query_size (InlineFragment _ q') := 1 + (query_set_size q');
-      query_size _ := 1
+      queries_size [::] := 0;
+      queries_size (cons hd tl) := query_size hd + queries_size tl
     }.
-  *)
-  Fixpoint query_set_size query_set : nat :=
-    match query_set with
-    | SingleQuery q => query_size q
-    | SelectionSet q q' => query_size q + query_set_size q'
-    end
-
-  with query_size query : nat :=
-         match query with
-         | NestedField _ _ q' => 1 + (query_set_size q')
-         | NestedLabeledField _ _ _ q' => 1 + (query_set_size q')
-         | InlineFragment _ q' => 1 + (query_set_size q')
-         | _ => 1
-         end.
-
-  Definition queries_size (queries : seq Query) := sumn (map query_size queries).
- 
 
   
   Definition partial_query_eq (q1 q2 : @Query Name Vals) : bool :=
@@ -62,19 +44,13 @@ Section QueryAux.
     | _, _ => false
     end.
 
-  Equations(noind) result_size result : nat :=
-    {
-      result_size (Results [::]) := 1;
-      result_size (Results (cons hd tl)) := 1 + (response_size hd) + (responses_size tl)
-    }
-  with
-  response_size response : nat :=
+  Equations(noind) response_size response : nat :=
     {
       response_size (Null _) := 3;
       response_size (SingleResult _ _) := 3;
       response_size (ListResult _ vals) := 4 + size vals;
-      response_size (NestedResult _ r') := 4 + result_size r';
-      response_size (NestedListResult _ rs) := 4 + 2 * size rs + results_size rs
+      response_size (NestedResult _ r') := 4 + responses_size r';
+      response_size (NestedListResult _ rs) := 4 + 2 * size rs + responses_size' rs
     }
   where
   responses_size (responses : seq (@ResponseObject Name Vals)) : nat :=
@@ -82,34 +58,19 @@ Section QueryAux.
       responses_size [::] := 0;
       responses_size (cons hd tl) := response_size hd + responses_size tl
     }
-  where
-  results_size (results : seq (@Result Name Vals)) : nat :=
+  where responses_size' (responses : seq (seq (@ResponseObject Name Vals))) : nat :=
     {
-      results_size [::] := 0;
-      results_size (cons hd tl) := (result_size hd) + (results_size tl)
+      responses_size' [::] := 0;
+      responses_size' (cons hd tl) := responses_size hd + responses_size' tl
     }.
-
-
-  
-  Fixpoint app_responses r1 r2 : @Result Name Vals :=
-    match r1, r2 with
-   | Results rs, Results rs' => Results (rs ++ rs')
-    end.
-
   
   Lemma responses_size_app (l1 l2 : seq.seq (@ResponseObject Name Vals)) : responses_size (l1 ++ l2) = responses_size l1 + responses_size l2.
-  Proof.
+  Proof. 
     elim: l1 => [//| n l' IH].
     by simpl; rewrite IH addnA.
   Qed.
   
-  Lemma responses_lt_result (l : list (@ResponseObject Name Vals)) (r : @Result Name Vals) :
-    responses_size l < result_size (Results l).
-  Proof.
-    elim: l => [| x l' IH].
-    - by simpl; rewrite result_size_equation_1.
-    - by simpl; rewrite result_size_equation_2;  ssromega.
-  Qed.
+  
 
   
   Lemma response_size_n_0 (r : @ResponseObject Name Vals) : 0 < response_size r.
